Partial bubble sort proof

theories/Sorted.v
@@ -4,4 +4,6 @@ Definition sorted {A : Type} (default : A) (compare : A -> A -> bool) (l : list 
 
 Definition prefixSorted {A : Type} (default : A) (compare : A -> A -> bool) (l : list A) (prefixLength : nat) := forall i j, i < j -> j < prefixLength -> ~compare (nth j l default) (nth i l default).
 
+Definition suffixSorted {A : Type} (default : A) (compare : A -> A -> bool) (l : list A) (suffixLength : nat) := forall i j, i < j -> length l - suffixLength <= i -> j < length l -> ~compare (nth j l default) (nth i l default).
+
 Definition partitioned {A : Type} (default : A) (compare : A -> A -> bool) (l : list A) (middle : nat) := forall toTheLeft toTheRight, toTheLeft <= middle -> toTheRight >= middle -> toTheRight < length l -> ~compare (nth toTheRight l default) (nth toTheLeft l default).
